research/rocket-verified-kernel/extracted/rocket_path_kernel.mli
@@ -1,0 +1,174 @@
+
+type bool =
+| True
+| False
+
+val negb : bool -> bool
+
+type nat =
+| O
+| S of nat
+
+type 'a option =
+| Some of 'a
+| None
+
+type ('a, 'b) prod =
+| Pair of 'a * 'b
+
+val fst : ('a1, 'a2) prod -> 'a1
+
+val snd : ('a1, 'a2) prod -> 'a2
+
+type 'a list =
+| Nil
+| Cons of 'a * 'a list
+
+val app : 'a1 list -> 'a1 list -> 'a1 list
+
+type comparison =
+| Eq
+| Lt
+| Gt
+
+val pred : nat -> nat
+
+module Nat :
+ sig
+  val sub : nat -> nat -> nat
+
+  val eqb : nat -> nat -> bool
+
+  val leb : nat -> nat -> bool
+
+  val ltb : nat -> nat -> bool
+
+  val compare : nat -> nat -> comparison
+
+  val divmod : nat -> nat -> nat -> nat -> (nat, nat) prod
+
+  val div : nat -> nat -> nat
+
+  val modulo : nat -> nat -> nat
+ end
+
+val map : ('a1 -> 'a2) -> 'a1 list -> 'a2 list
+
+val seq : nat -> nat -> nat list
+
+val rev : 'a1 list -> 'a1 list
+
+val filter : ('a1 -> bool) -> 'a1 list -> 'a1 list
+
+module PathModel :
+ sig
+  type target =
+  | Origin of nat
+  | Complete
+
+  val labels : nat -> nat list
+
+  val valid_label : nat -> nat -> bool
+
+  val lookup_nat : nat -> (nat, nat) prod list -> nat option
+
+  val update_nat : nat -> nat -> (nat, nat) prod list -> (nat, nat) prod list
+
+  val member_nat : nat -> nat list -> bool
+
+  val digits_rev_fuel : nat -> nat -> nat list
+
+  val digits_rev : nat -> nat list
+
+  val decimal_digits : nat -> nat list
+
+  val compare_digits : nat list -> nat list -> comparison
+
+  val compare_encoded_int : nat -> nat -> comparison
+
+  val encoded_int_lt : nat -> nat -> bool
+
+  type successor_table = (nat, target) prod list
+
+  type solver_state = { st_size : nat; st_entry : nat;
+                        st_edges : successor_table;
+                        st_predecessors : nat list;
+                        st_parent : (nat, nat) prod list;
+                        st_components : nat; st_terminal : nat option }
+
+  val st_size : solver_state -> nat
+
+  val st_entry : solver_state -> nat
+
+  val st_edges : solver_state -> successor_table
+
+  val st_predecessors : solver_state -> nat list
+
+  val st_parent : solver_state -> (nat, nat) prod list
+
+  val st_components : solver_state -> nat
+
+  val st_terminal : solver_state -> nat option
+
+  val make_state :
+    nat -> nat -> successor_table -> nat list -> (nat, nat) prod list -> nat
+    -> nat option -> solver_state
+
+  val initial_state : nat -> nat -> solver_state
+
+  val dsu_find_fuel : nat -> nat -> (nat, nat) prod list -> nat
+
+  val dsu_find : nat -> nat -> (nat, nat) prod list -> nat
+
+  val dsu_union :
+    nat -> nat -> nat -> (nat, nat) prod list -> (nat, nat) prod list option
+
+  val state_with_edge :
+    solver_state -> nat -> target -> nat list -> (nat, nat) prod list -> nat
+    -> nat option -> solver_state
+
+  val try_origin : solver_state -> nat -> nat -> solver_state option
+
+  val try_complete : solver_state -> nat -> solver_state option
+
+  val try_target : solver_state -> nat -> target -> solver_state option
+
+  val partial_state_feasible : solver_state -> nat -> bool
+
+  val insert_encoded : nat -> nat list -> nat list
+
+  val sort_encoded : nat list -> nat list
+
+  val candidate_labels : solver_state -> nat list -> nat list
+
+  val ordered_candidates : solver_state -> nat list -> target list
+
+  val choose_candidate :
+    nat -> solver_state -> nat -> nat -> target list -> solver_state option
+
+  val process_sources :
+    nat -> nat -> nat list -> solver_state -> solver_state option
+
+  val minimum_encoded_aux : nat -> nat list -> nat
+
+  val minimum_encoded_label : nat -> nat
+
+  val canonical_state : nat -> solver_state option
+
+  val lookup_successor : nat -> (nat, target) prod list -> target option
+
+  val follow_aux :
+    nat -> nat -> nat list -> (nat, target) prod list -> nat list -> nat list
+    option
+
+  val canonical_labels : nat -> nat list
+
+  val canonical_successors : nat -> successor_table
+ end
+
+module PathCanon :
+ sig
+  val canonical_assignment : nat -> nat list
+
+  val induced_successors : nat -> PathModel.successor_table
+ end
